MCInstances.v
@@ -1,0 +1,17 @@
+Require Import MathClasses.interfaces.canonical_names.
+Require Import CanonicalNotations.
+Require Export core.
+Instance Zero_instance_QTime : Zero QTime := (mkQTime 0 I).
+Instance Zero_instance_Time : Zero Time := (QT2T (mkQTime 0 I)).
+Instance Zero_instance_IR : Zero IR := [0]. (** why not prove it is a ring *)
+
+Instance SqrtFun_instancee_IR : SqrtFun IR IR.
+intros r. apply (sqrt (AbsIR r)). apply AbsIR_nonneg.
+Defined.
+
+Instance Plus_instance_IR : Plus IR := csg_op .
+Instance Mult_instance_IR : Mult IR := cr_mult.
+Instance Negate_instance_IR : Negate IR := cg_inv.
+Instance Cast_instace_Q_IR : Cast Q IR := (inj_Q IR).
+(* Instance Lt_instace_Q_IR : Lt IR.
+  intros a b. *)
